001-separate-paren-groups.dfy
@@ -1,59 +1,104 @@
-function IsValidParentheses(s: string, i: int, depth: int): bool
-  decreases |s| - i
-  requires 0 <= i && i <= |s|
+function ParenthesesDepth(s: string, i: int, j: int): int
+    decreases j - i 
+    requires 0 <= i <= j <= |s|
 {
-    if i == |s| then
-        depth >= 0
-    else if depth < 0 then
-        false
+    if i == j then
+        0
     else if s[i] == '(' then
-        IsValidParentheses(s, i + 1, depth + 1)
+        ParenthesesDepth(s, i+1, j) + 1
     else if s[i] == ')' then
-        depth > 0 && IsValidParentheses(s, i + 1, depth - 1)
+        ParenthesesDepth(s, i+1, j) - 1
     else
-        IsValidParentheses(s, i + 1, depth)
+        ParenthesesDepth(s, i+1, j)
 }
 
-function IsValidParentheses2(s: string, i: int, depth: int): bool
-  decreases |s| - i
-  requires 0 <= i && i <= |s|
+predicate InnerDepthsPositive(s: string)
 {
-    if i == |s| then
-        depth == 0
-    else if depth < 0 then
-        false
-    else if s[i] == '(' then
-        IsValidParentheses2(s, i + 1, depth + 1)
-    else if s[i] == ')' then
-        if depth > 0 then IsValidParentheses2(s, i + 1, depth - 1) else false
-    else
-        IsValidParentheses2(s, i + 1, depth)
+    forall i :: 0 < i < |s| ==> ParenthesesDepth(s, 0, i) > 0
 }
 
-function IsValidParentheses1(s: string, i: int, depth: int): bool
-  decreases |s| - i
-  requires 0 <= i && i <= |s|
+predicate InnerDepthsNonnegative(s: string)
 {
-    if i == |s| then
-        depth == 0
-    else if (depth <= 0 && i != 0) then
-        false
-    else if s[i] == '(' then
-        IsValidParentheses1(s, i + 1, depth + 1)
-    else if s[i] == ')' then
-        depth > 0 && IsValidParentheses1(s, i + 1, depth - 1)
-    else
-        IsValidParentheses1(s, i + 1, depth)
+    forall i :: 0 < i < |s| ==> ParenthesesDepth(s, 0, i) >= 0
+}
+
+lemma ParenthesesDepthSum(s: string, i: int, j: int, k: int)
+    decreases j - i
+    requires 0 <= i <= j <= k <= |s|
+    ensures ParenthesesDepth(s, i, k) == ParenthesesDepth(s, i, j) + ParenthesesDepth(s, j, k)
+{
+    if i != j {
+        ParenthesesDepthSum(s, i+1, j, k);
+    }
+}
+
+lemma ParenthesesSuffixEq(s: string, i: int, j: int)
+    decreases j -i
+    requires 0 <= i <= j <= |s|
+    ensures ParenthesesDepth(s, i, j) == ParenthesesDepth(s[..j], i, j)
+{
+    if i != j {
+        ParenthesesSuffixEq(s, i+1, j);
+    }
+}
+
+lemma ParenthesesPrefixEq(s: string, i: int, j: int)
+    decreases j -i
+    requires 0 <= i <= j <= |s|
+    ensures ParenthesesDepth(s, i, j) == ParenthesesDepth(s[i..], 0, j-i)
+{ }
+
+lemma ParenthesesSubstring(s: string, i: int, j: int)
+    decreases j - i
+    requires 0 <= i <= j <= |s|
+    ensures ParenthesesDepth(s, i, j) == ParenthesesDepth(s[i..j], 0, j-i)
+{
+    assert ParenthesesDepth(s, i, j) == ParenthesesDepth(s[..j], i, j)
+        by { ParenthesesSuffixEq(s, i, j); }
+    assert ParenthesesDepth(s[..j], i, j) == ParenthesesDepth(s[i..j], 0, j-i)
+        by { ParenthesesPrefixEq(s[..j], i, j); }
+}
+
+lemma ParenthesesCommonSegment(s: string, t: string, i: int, j: int)
+    requires 0 <= i <= j <= |s|
+    requires 0 <= i <= j <= |t|
+    requires s[i..j] == t[i..j]
+    ensures ParenthesesDepth(s, i, j) == ParenthesesDepth(t, i, j)
+{
+    ParenthesesSubstring(s, i, j);
+    ParenthesesSubstring(t, i, j);
+}
+
+lemma ParenthesesDepthAppend(s: string, c: char)
+    ensures ParenthesesDepth(s + [c], 0, |s|+1) == ParenthesesDepth(s, 0, |s|) + ParenthesesDepth([c], 0, 1)
+{
+    ParenthesesSubstring(s + [c], 0, |s|);
+    ParenthesesSubstring(s + [c], |s|, |s| + 1);
+    ParenthesesDepthSum(s + [c], 0, |s|, |s| + 1);
+}
+
+lemma InnerDepthsPositiveAppendDecompose(s: string, c: char)
+    requires InnerDepthsPositive(s)
+    requires ParenthesesDepth(s, 0, |s|) > 0
+    ensures InnerDepthsPositive(s + [c])
+{
+    forall i: int | 0 < i < |s| + 1
+        ensures ParenthesesDepth(s + [c], 0, i) > 0
+    {
+        if (i <= |s|) {
+            ParenthesesCommonSegment(s, s + [c], 0, i);
+        }
+    }
 }
 
 method separate_paren_groups(paren_string: string) returns (res : seq<string>)
     // pre-conditions-start
-    requires forall i :: i >= 0 && i < |paren_string| ==> paren_string[i] == '(' || paren_string[i] == ')'
-    requires forall i :: 0 <= i <= |paren_string| ==> IsValidParentheses(paren_string, i, 0)
-    requires IsValidParentheses2(paren_string, 0, 0)
+    requires ParenthesesDepth(paren_string, 0, |paren_string|) == 0
+    requires InnerDepthsNonnegative(paren_string)
     // pre-conditions-end
     // post-conditions-start
-    ensures |res| > 0 ==> forall i :: 0 <= i < |res| ==> IsValidParentheses1(res[i], 0, 0)
+    ensures forall k :: 0 <= k < |res| ==> ParenthesesDepth(res[k], 0, |res[k]|) == 0
+    ensures forall k :: 0 <= k < |res| ==> InnerDepthsPositive(res[k])
     // post-conditions-end
 {
     // impl-start
@@ -65,13 +110,29 @@ method separate_paren_groups(paren_string: string) returns (res : seq<string>)
 
     while (i < |paren_string|)
         // invariants-start
-        invariant 0 <= i && i <= |paren_string|
-        invariant 0 <= i && i < |paren_string| ==> paren_string[i] in {'(', ')'}
-        invariant |res| > 0 ==> (forall i1 :: 0 <= i1 < |res| ==> IsValidParentheses1(res[i1], 0, 0))
-        invariant IsValidParentheses(paren_string, i, 0)
+        invariant 0 <= i <= |paren_string|
+        invariant forall k :: 0 <= k < |res| ==> ParenthesesDepth(res[k], 0, |res[k]|) == 0
+        invariant forall k :: 0 <= k < |res| ==> InnerDepthsPositive(res[k])
+        invariant ParenthesesDepth(paren_string, 0, |paren_string|) == 0
+        invariant InnerDepthsNonnegative(paren_string)
+        invariant ParenthesesDepth(paren_string, i, |paren_string|) + current_depth == 0
+        invariant ParenthesesDepth(paren_string, 0, i) == current_depth
+        invariant ParenthesesDepth(current_string, 0, |current_string|) == current_depth
+        invariant InnerDepthsPositive(current_string)
+        invariant current_string == "" || current_depth > 0
+        invariant current_depth >= 0
         // invariants-end
     {
         var c: char := paren_string[i];
+
+        // lemma-use-start
+        ParenthesesDepthAppend(current_string, c);
+        ParenthesesDepthSum(paren_string, 0, i, i+1);
+        if (current_string != "") {
+            InnerDepthsPositiveAppendDecompose(current_string, c);
+        }
+        // lemma-use-end
+
         if (c == '(')
         {
             current_depth := current_depth + 1;
